LabSession06_File.v
@@ -1,0 +1,232 @@
+Require Import TacticsL8 Maps Arith.
+Open Scope nat_scope.
+
+
+(* ================================================================= *)
+(** ** Arithmetic and Boolean Expressions *)
+(* We start by defining types for arithmetic and boolean
+   expressions. Since we are interested in having
+   expressions with variables, we also need the notion
+   of state. *)
+
+Definition state := total_map nat.
+
+Inductive aexp : Type :=
+  | ANum (n : nat)
+  | AId (x : string)
+  | APlus (a1 a2 : aexp)
+  | AMinus (a1 a2 : aexp)
+  | AMult (a1 a2 : aexp).
+
+(** Defining a few variable names as notational shorthands will make
+    examples easier to read: *)
+
+Definition W : string := "W".
+Definition X : string := "X".
+Definition Y : string := "Y".
+Definition Z : string := "Z".
+
+Inductive bexp : Type :=
+  | BTrue
+  | BFalse
+  | BEq (a1 a2 : aexp)
+  | BLe (a1 a2 : aexp)
+  | BNot (b : bexp)
+  | BAnd (b1 b2 : bexp).
+
+Coercion AId : string >-> aexp.
+Coercion ANum : nat >-> aexp.
+
+Definition bool_to_bexp (b : bool) : bexp :=
+  if b then BTrue else BFalse.
+Coercion bool_to_bexp : bool >-> bexp.
+
+Bind Scope imp_scope with aexp.
+Bind Scope imp_scope with bexp.
+Delimit Scope imp_scope with imp.
+
+Notation "x + y" := (APlus x y) (at level 50, left associativity) : imp_scope.
+Notation "x - y" := (AMinus x y) (at level 50, left associativity) : imp_scope.
+Notation "x * y" := (AMult x y) (at level 40, left associativity) : imp_scope.
+Notation "x <= y" := (BLe x y) (at level 70, no associativity) : imp_scope.
+Notation "x = y" := (BEq x y) (at level 70, no associativity) : imp_scope.
+Notation "x && y" := (BAnd x y) (at level 40, left associativity) : imp_scope.
+Notation "'~' b" := (BNot b) (at level 75, right associativity) : imp_scope.
+
+(** We can now write [3 + (X * 2)] instead  of [APlus 3 (AMult X 2)],
+    and [true && ~(X <= 4)] instead of [BAnd true (BNot (BLe X 4))]. *)
+
+Definition example_aexp := (3 + (X * 2))%imp : aexp.
+Definition example_bexp := (true && ~(X <= 4))%imp : bexp.
+
+(** One downside of these coercions is that they can make it a little
+    harder for humans to calculate the types of expressions.  If you
+    get confused, try doing [Set Printing Coercions] to see exactly
+    what is going on. *)
+
+Print example_bexp.
+Set Printing Coercions. 
+(* In CoqIDE, this might have to be set in the View menu *)
+
+Print example_bexp.
+(* ===> example_bexp = bool_to_bexp true && ~ (AId X <= ANum 4) *)
+
+Unset Printing Coercions.
+
+(* ================================================================= *)
+(** ** Functional Evaluation *)
+
+Fixpoint aeval (st : state) (a : aexp) : nat :=
+  match a with
+  | ANum n => n
+  | AId x => st x
+  | APlus a1 a2 => (aeval st a1) + (aeval st a2)
+  | AMinus a1 a2  => (aeval st a1) - (aeval st a2)
+  | AMult a1 a2 => (aeval st a1) * (aeval st a2)
+  end.
+
+Fixpoint beval (st : state) (b : bexp) : bool :=
+  match b with
+  | BTrue       => true
+  | BFalse      => false
+  | BEq a1 a2   => (aeval st a1) =? (aeval st a2)
+  | BLe a1 a2   => (aeval st a1) <=? (aeval st a2)
+  | BNot b1     => negb (beval st b1)
+  | BAnd b1 b2  => andb (beval st b1) (beval st b2)
+  end.
+
+Definition empty_st := t_empty 0.
+
+(** Now we can add a notation for a "singleton state" with just one
+    variable bound to a value. *)
+Notation "a '!->' x" := (t_update empty_st a x) (at level 100).
+
+Example aexp1 :
+    aeval (X !-> 5) (3 + (X * 2))%imp
+  = 13.
+Proof. reflexivity. Qed.
+
+Example bexp1 :
+    beval (X !-> 5) (true && ~(X <= 4))%imp
+  = true.
+Proof. reflexivity. Qed.
+
+(* ================================================================= *)
+(** ** Relational Evaluation *)
+
+Reserved Notation "st '|-' e '\\' n"
+                  (at level 90, left associativity).
+
+Inductive aevalR : aexp -> state -> nat -> Prop :=
+| E_ANum (n: nat) : forall st,
+    st |- (ANum n) \\ n
+| E_AId (x: string) : forall st v,
+    st x = v ->
+    st |- (AId x) \\ v
+| E_APlus (a1 a2: aexp) : forall st n1 n2 n3,
+    st |- a1 \\ n1 ->
+    st |- a2 \\ n2 ->
+    (n1 + n2)%nat = n3 ->
+    st |- APlus a1 a2 \\ n3
+| E_AMinus (a1 a2: aexp) : forall st n1 n2 n3,
+    st |- a1 \\ n1 ->
+    st |- a2 \\ n2 ->
+    (n1 - n2)%nat = n3 ->
+    st |- AMinus a1 a2 \\ n3
+| E_AMult (a1 a2: aexp) : forall st n1 n2 n3,
+    st |- a1 \\ n1 ->
+    st |- a2 \\ n2 ->
+    (n1 * n2)%nat = n3 ->
+    st |- AMult a1 a2 \\ n3
+
+where "st '|-' e '\\' n" := (aevalR e st n) : type_scope.
+
+
+(* TODO: exercises 1.2 and 1.4 *)
+
+
+(* ================================================================= *)
+(** ** Imperative Programs *)
+
+(* We now define a small imperative language with While loops *)
+
+Module WhileLoops.
+ Inductive com : Type :=
+  | CSkip
+  | CAss (x : string) (a : aexp)
+  | CSeq (c1 c2 : com)
+  | CIf (b : bexp) (c1 c2 : com)
+  | CWhile (b : bexp) (c : com).
+
+(* We define some notation *)
+Bind Scope imp_scope with com.
+Notation "'SKIP'" :=
+   CSkip : imp_scope.
+Notation "x '::=' a" :=
+  (CAss x a) (at level 60) : imp_scope.
+Notation "c1 ;; c2" :=
+  (CSeq c1 c2) (at level 80, right associativity) : imp_scope.
+Notation "'WHILE' b 'DO' c 'END'" :=
+  (CWhile b c) (at level 80, right associativity) : imp_scope.
+Notation "'TEST' c1 'THEN' c2 'ELSE' c3 'FI'" :=
+  (CIf c1 c2 c3) (at level 80, right associativity) : imp_scope.
+
+Open Scope imp_scope.
+
+Example prog2 := WHILE (X <= 2) DO (Y ::= Y + 1 ;; X ::= X - 1) END.
+
+Definition fact_in_coq : com :=
+  (Z ::= X;;
+  Y ::= 1;;
+  WHILE ~(Z = 0) DO
+    Y ::= Y * Z;;
+    Z ::= Z - 1
+  END)%imp.
+
+Open Scope imp_scope.
+
+Fixpoint exec (st : state) (c : com): state :=
+  match c with
+    | SKIP =>  st 
+    | x ::= a1 => st & {x --> (aeval st a1)}
+    | c1 ;; c2 => let st' := exec st c1
+                 in   exec st' c2
+    | TEST b THEN c1 ELSE c2 FI => if (beval st b)
+                                  then exec st c1
+                                  else exec st c2
+    | WHILE b DO c END => st  (* DOES NOTHING!! *)
+  end.
+Close Scope imp_scope.
+
+(* Defining the semantics of while loops functionally can cause
+   some problems, so now we do it relationally *)
+
+Reserved Notation "st '=[' c ']=>' st'"
+                  (at level 40).
+
+
+(* TODO: exercise 1.5 *)
+Inductive ceval : com -> state -> state -> Prop :=
+  | E_Skip : forall st,
+      (*TODO*)
+  | E_Ass  : forall st a1 n x,
+      aeval st a1 = n ->
+      (*TODO*)
+  | E_Seq : forall c1 c2 st st' st'',
+      (*TODO*)
+  | E_IfTrue : forall st st' b c1 c2,
+      beval st b = true ->
+      (*TODO*)
+  | E_IfFalse : forall st st' b c1 c2,
+      beval st b = false ->
+      (*TODO*)
+  | E_WhileFalse : forall b st c,
+      beval st b = false ->
+      (*TODO*)
+  | E_WhileTrue : forall st st' st'' b c,
+      beval st b = true ->
+      (*TODO*)
+
+  where "st =[ c ]=> st'" := (ceval c st st').
+       
+End WhileLoops.
