Lecture11_live.v
@@ -1,0 +1,290 @@
+Require Import Maps TacticsL8 String.
+
+Notation var := string.
+Definition valuation := partial_map nat.
+
+Example m1 := empty & {{ "x" --> 0}}.
+(*
+d = {}
+d['x'] = 0
+*)
+Compute m1 "x".
+Compute m1 "y".
+Example m2 := m1 & {{ "x" --> 1 }}.
+Compute m2 "x".
+
+Inductive arith : Type :=
+  | Const (n : nat)
+  | Var (x : var)
+  | Plus (e1 e2: arith)
+  | Minus (e1 e2: arith)
+  | Times (e1 e2: arith).
+
+Fixpoint interp (e:arith) (v:valuation) : nat :=
+  match e with
+  | Const n => n
+  | Var x => match v x with
+            | None => 0
+            | Some n => n
+            end
+  | Plus e1 e2 => interp e1 v  +  interp e2 v
+  | Minus e1 e2 => interp e1 v  -  interp e2 v
+  | Times e1 e2 => interp e1 v  *  interp e2 v
+  end.
+
+Example ex1 := Plus (Const 1) 
+                    (Times (Const 2)  (Const 3)). (* 7 *)
+
+Example ex2 := Plus (Const 1) 
+                    (Times (Const 2)  (Var "x")).
+Compute interp ex2 m2.
+
+Fixpoint doSomeArithmetic (e:arith) : arith :=
+  match e with
+  | Const _ => e
+  | Var _ => e
+  | Plus (Const n1) (Const n2) => Const (n1+n2)
+  | Times (Const n1) (Const n2) => Const (n1*n2)
+  | Plus e1 e2 => Plus (doSomeArithmetic e1)
+                       (doSomeArithmetic e2)
+  | Minus e1 e2 => Minus (doSomeArithmetic e1)
+                         (doSomeArithmetic e2)
+  | Times e1 e2 => Times (doSomeArithmetic e1)
+                         (doSomeArithmetic e2)
+  end.
+
+Print ex1.
+Compute doSomeArithmetic ex1.
+
+Inductive instruction :=
+ | PushConst (n : nat)
+ | PushVar (x : var)
+ | Add
+ | Subtract
+ | Multiply.
+
+Definition run1 (i:instruction) (v:valuation) 
+                (stack: list nat) : list nat :=
+  match i with
+  | PushConst n => n :: stack
+  | PushVar x   => (match v x with
+                   | None => 0
+                   | Some n => n
+                   end) :: stack
+  | Add => match stack with
+           | n1 :: n2 :: stack' => n2+n1 :: stack'
+           | _                  => stack
+          end
+  | Subtract => match stack with
+                | n1 :: n2 :: stack' => n2-n1 :: stack'
+                | _                  => stack
+                end
+  | Multiply => match stack with
+                | n1 :: n2 :: stack' => n2*n1 :: stack'
+                | _                  => stack
+                end
+  end.
+
+Example i1 := [ PushConst 1; PushConst 2; Add ].
+Example valuation0 := empty & {{ "x" --> 1 }}.
+
+(** This is where we stopped in Lecture 10 *)
+(** We will continue from here in Lecture 11 *)
+
+(** TODO: define run *)
+Fixpoint run (is : list instruction) (v: valuation) 
+             (stack : list nat) : list nat :=
+  match is with
+  | []   => stack  (* no state changes *)
+  | i::t => run t v (run1 i v stack)
+  end.
+
+Example i2 := [ PushConst 1; PushConst 2; Add; PushConst 4; Add ].
+
+Compute run i2 valuation0 [].
+
+
+(** TODO: define compile *)
+Fixpoint compile (e:arith) : list instruction :=
+  match e with
+  | Const n    => [PushConst n]
+  | Var x      => [PushVar x]
+  | Plus e1 e2 => (compile e1)  ++ (compile e2) ++ [Add]
+  | Minus e1 e2 => (compile e1) ++ (compile e2) ++ [Subtract]
+  | Times e1 e2 => (compile e1) ++ (compile e2) ++ [Multiply]
+  end.
+
+Example exp1 := Times (Plus (Const 1) (Const 2)) (Minus (Const 3) (Var "x")).
+
+Example exp2 := Times exp1 exp1.
+
+Compute compile exp2.
+
+
+Lemma compile_ok' : forall e v is stack,
+    run (compile e ++ is) v stack = run is v (interp e v :: stack).
+Proof.
+  induction e; intros; simpl.
+  - equality.
+  - equality.
+  - rewrite app_assoc_reverse. rewrite app_assoc_reverse.
+    rewrite IHe1.
+    rewrite IHe2. simpl. equality.
+  - try repeat rewrite app_assoc_reverse.
+    rewrite IHe1. rewrite IHe2. simpl. equality.
+  - try repeat rewrite app_assoc_reverse.
+    rewrite IHe1. rewrite IHe2. simpl. equality.
+Qed.
+
+(*
+Theorem compile_ok : forall e v,
+    run (compile e) v nil = interp e v :: nil.
+Proof.
+  intros. simpl.
+  (* To match the form of our lemma, we need to replace [compile e] with
+   * [compile e ++ nil], adding a "pointless" concatenation of the empty list.
+   * [SearchRewrite] helps us find a library lemma. *)
+  rewrite (app_nil_end (compile e)).
+  (* Note that we can use [rewrite] with explicit values of the first few
+   * quantified variables of a lemma.  Otherwise, [rewrite] picks an
+   * unhelpful place to rewrite.  (Try it and see!) *)
+  apply compile_ok'.
+  (* Direct appeal to a previously proved lemma *)
+Qed.
+*)
+
+Inductive logic : Type :=
+| bTrue
+| bFalse
+| Not (l:logic)
+| Conjuction (l1 l2:logic)
+| Le (a1 a2:arith).
+
+Fixpoint bInterp (e:logic) (v:valuation) : bool :=
+match e with
+| bTrue => true
+| bFalse => false
+| Not l => negb (bInterp l v)
+| Conjuction l1 l2 => andb (bInterp l1 v) (bInterp l2 v)
+| Le a1 a2 => leb (interp a1 v) (interp a2 v)
+end.
+
+Inductive cmd : Type :=
+  | Skip   (* No op command *)
+  | Assign (x : var) (e : arith)
+  | Sequence (c1 c2 : cmd)
+  | Repeat (e : arith) (body : cmd)
+  | If (b : logic) (t e: cmd).
+
+Example prog1 :=
+  Sequence (Assign "x" (Const 1)) (Assign "y" (Const 2)).
+(* This is the same as x <- 1; y <- 2 *)
+
+(** The function selfCompose will be helpful when 
+    defining evaluation for our tiny imperative
+    language. This function corresponds to repeated
+    application of a function. *)
+Fixpoint selfCompose {A} (f : A -> A) (n : nat) : A -> A :=
+  match n with
+  | O => fun x => x
+  | S n' => fun x => selfCompose f n' (f x)
+  end.
+
+Fixpoint exec (c:cmd) (v:valuation) : valuation :=
+  match c with
+  | Skip            =>  v
+  | Assign x e      =>  v & {{ x --> interp e v }}
+  | Sequence c1 c2  =>  exec c2 (exec c1 v)
+  | Repeat e body   =>  selfCompose (exec body) (interp e v) v
+  | If t b1 b2      => if (bInterp t v) then exec b1 v else exec b2 v
+  end.
+
+Definition bool2logic (b:bool) : logic :=
+match b with
+| true => bTrue
+| false => bFalse
+end.
+
+(** The following notations will be helpful later *)
+Coercion Const : nat >-> arith.
+Coercion Var : var >-> arith.
+Coercion bool2logic : bool >-> logic.
+Infix "+" := Plus : arith_scope.
+Infix "-" := Minus : arith_scope.
+Infix "*" := Times : arith_scope.
+Infix "&&" := Conjuction : logic_scope.
+Delimit Scope arith_scope with arith.
+Delimit Scope logic_scope with logic.
+Notation "x <- e" := (Assign x e%arith) (at level 75).
+Infix ";" := Sequence (at level 76).
+Notation "'repeat' e 'doing' body 'done'" := (Repeat e%arith body) (at level 75).
+Notation "'testing' t 'do' b1 'or' b2 'cond'" := (If t%logic b1 b2).
+Notation "'not' b" := (Not b%logic) (at level 75).
+
+Lemma ifTrue: forall t b1 b2 v,
+  (bInterp t v) = true -> exec (If t b1 b2) v = exec b1 v.
+Proof.
+intros. simpl. rewrite H. easy. Qed.
+
+Lemma ifFalse: forall t b1 b2 v,
+  (bInterp t v) = false -> exec (If t b1 b2) v = exec b2 v.
+Proof.
+intros. simpl. rewrite H. easy. Qed.
+
+Lemma ifOneOrOther: forall t b1 b2 v,
+  exec (If t b1 b2) v = exec b1 v \/ exec (If t b1 b2) v = exec b2 v.
+Proof.
+intros. simpl. destruct bInterp.
+ - left. easy.
+ - right. easy.
+Qed.
+
+(** Properties *)
+
+Lemma cmd_seq_assoc: forall c1 c2 c3 v,
+    exec ((c1 ; c2 ) ; c3)  v = exec (c1 ; (c2 ; c3)) v.
+Proof.
+  intros; induction c1; simpl; reflexivity.
+Qed.  
+
+Lemma cmd_seq_skip_r: forall c v,
+    exec (c ; Skip) v = exec c v.
+Proof.
+  reflexivity.
+Qed.
+
+Lemma cmd_seq_skip_l: forall c v,
+    exec (Skip ; c) v = exec c v.
+Proof.
+  reflexivity.
+Qed.
+
+
+Lemma cmd_no_repeat: forall c v,
+    exec (repeat 0 doing c done) v = exec Skip v.
+Proof. 
+  reflexivity. 
+Qed.
+
+Lemma cmd_seq: forall c1 c2 v,
+    exec (c1 ; c2) v = exec c2 (exec c1 v).
+Proof.
+  reflexivity.
+Qed.
+
+Lemma selfCompose_n: forall A (f:A->A) n v,
+    selfCompose f (n+1) v = selfCompose f n (f v).
+Proof.
+  induction n.
+  - simpl. reflexivity.
+  - intros. simpl. rewrite IHn. reflexivity.
+Qed.
+
+Lemma cmd_repeat_unroll: forall c1 v (n:nat),
+          exec (repeat (n+1) doing c1 done) v
+        = exec (c1; repeat n doing c1 done) v.
+Proof.
+  induction n.
+  - simpl. reflexivity.
+  - rewrite cmd_seq. simpl in *. apply selfCompose_n.
+Qed.
